Remove TFRAME from the world, WIP to create the continuation relation

theories/logrel.v
@@ -35,21 +35,23 @@ Section logrel.
     {Σ:gFunctors}
     {ceriseg:ceriseG Σ} {sealsg: sealStoreG Σ}
     {Cname : CmptNameG}
-    {stsg : STSG Addr region_type Σ} {tframeg : TFRAMEG Σ} {heapg : heapGS Σ}
+    {stsg : STSG Addr region_type Σ} {heapg : heapGS Σ}
     {nainv: logrel_na_invs Σ}
     `{MP: MachineParameters}.
 
   Notation STS := (leibnizO (STS_states * STS_rels)).
   Notation STS_STD := (leibnizO (STS_std_states Addr region_type)).
-  Notation TFRAME := (leibnizO nat).
-  Notation WORLD := ( prodO (prodO STS_STD STS) TFRAME) .
+  Notation WORLD := (prodO STS_STD STS).
+  Notation STK := (leibnizO (list (iProp Σ * Word * Word))).
   Implicit Types W : WORLD.
   Implicit Types C : CmptName.
 
-  Notation D := (WORLD -n> (leibnizO CmptName) -n> (leibnizO Word) -n> iPropO Σ).
+  Notation E := (STK -n> WORLD -n> (leibnizO CmptName) -n> (leibnizO Word) -n> (leibnizO Word) -n> iPropO Σ).
+  Notation V := (WORLD -n> (leibnizO CmptName) -n> (leibnizO Word) -n> iPropO Σ).
+  Notation K := (STK -n> WORLD -n> (leibnizO CmptName) -n> iPropO Σ).
   Notation R := (WORLD -n> (leibnizO CmptName) -n> (leibnizO Reg) -n> iPropO Σ).
   Implicit Types w : (leibnizO Word).
-  Implicit Types interp : (D).
+  Implicit Types interp : (V).
 
   (* -------------------------------------------------------------------------------- *)
 
@@ -92,7 +94,7 @@ Section logrel.
     ([∗ map] r↦w ∈ r, r ↦ᵣ w)%I.
 
   Definition full_map (reg : Reg) : iProp Σ := (∀ (r : RegName), ⌜is_Some (reg !! r)⌝)%I.
-  Program Definition interp_reg (interp : D) : R :=
+  Program Definition interp_reg (interp : V) : R :=
     λne (W : WORLD) (C : CmptName) (reg : leibnizO Reg),
       (full_map reg ∧
        ∀ (r : RegName) (v : Word), (⌜r ≠ PC⌝ → ⌜reg !! r = Some v⌝ → interp W C v))%I.
@@ -113,77 +115,121 @@ Section logrel.
     (WP Seq (Instr Executable)
        {{ v, ⌜v = HaltedV⌝ → na_own logrel_nais ⊤ }})%I.
 
-  Program Definition interp_expr (interp : D) (regs : Reg) : D :=
-    (λne (W : WORLD) (C : CmptName) (w : Word),
+
+
+  Program Definition interp_expr (interp : V) (interp_cont : K) : E :=
+    (λne (stk : STK) (W : WORLD) (C : CmptName) (wpc : Word) (wstk : Word),
+       ∀ regs,
        ( interp_reg interp W C regs
-        ∗ registers_pointsto (<[PC:=w]> regs)
+        ∗ registers_pointsto (<[PC:=wpc]> (<[csp:=wpc]> regs))
         ∗ region W C
         ∗ sts_full_world W C
-        ∗ tframe_frag (frm W)
-        ∗ na_own logrel_nais ⊤
+        ∗ interp_cont stk W C
+        (* ∗ na_own logrel_nais ⊤ *)
           -∗ interp_conf W C)
     )%I.
   Solve All Obligations with solve_proper.
 
+  Program Definition interp_cont (interp : V) (interp_cont : K) : K :=
+    λne (stk : STK) (W : WORLD) (C : CmptName),
+    (match stk with
+    | [] => False%I
+    | (P,wret,wstk)::stk' =>
+      (□ (∀ W', ⌜related_sts_pub_world W W'⌝ -∗
+               P -∗ ▷ interp_expr interp interp_cont stk' W' C wret wstk
+        ))%I
+     end
+    ).
+  Solve All Obligations with solve_proper.
+
+  Global Instance interp_continuation_ne (interp : V) n :
+    Proper (dist n ==> dist n) (interp_cont interp).
+  Proof. unfold interp_cont. solve_proper.
+         destruct x0; first done.
+         destruct p.
+         destruct p.
+         solve_proper.
+  Qed.
+  Global Instance interp_cont_contractive (interp : V) :
+    Contractive (λ interp_cont', (interp_cont interp) interp_cont').
+  Proof.
+    solve_proper_prepare.
+    destruct x0; first done.
+    destruct p.
+    destruct p.
+    solve_contractive.
+  Qed.
+
+  (* Lemma fixpoint_interp_continuation_eq (interp : V) (stk : STK) (W : WORLD) (C : CmptName) (w : leibnizO Word) : *)
+  (*   fixpoint (interp_continuation interp) stk W C ≡ interp_continuation interp (fixpoint (interp_continuation interp)) stk W C. *)
+  (* Proof. exact: (fixpoint_unfold (interp_continuation interp) stk W C). Qed. *)
+
+  (* Definition interp_cont (interp : V) := fixpoint (interp_continuation interp). *)
+  (* Definition interp_expr (interp : V) := interp_expr' interp (interp_cont interp). *)
+
   (* Condition definitions *)
-  Definition zcond (P : D) (C : CmptName) : iProp Σ :=
+  Definition zcond (P : V) (C : CmptName) : iProp Σ :=
     (□ ∀ (W1 W2: WORLD) (z : Z), P W1 C (WInt z) -∗ P W2 C (WInt z)).
   Global Instance zcond_ne n :
     Proper ((=) ==> (=) ==> dist n) zcond.
   Proof. solve_proper_prepare.
          repeat f_equiv;auto. Qed.
-  Global Instance zcond_contractive (P : D) (C : CmptName) :
+  Global Instance zcond_contractive (P : V) (C : CmptName) :
     Contractive (λ interp, ▷ zcond P C)%I.
   Proof. solve_contractive. Qed.
 
-  Definition rcond (P : D) (C : CmptName) (p : Perm) (interp : D) : iProp Σ :=
+  Definition rcond (P : V) (C : CmptName) (p : Perm) (interp : V) : iProp Σ :=
     (□ ∀ (W: WORLD) (w : Word), P W C w -∗ interp W C (load_word p w)).
   Global Instance rcond_ne n :
     Proper ((=) ==> (=) ==> (=) ==> dist n ==> dist n) rcond.
   Proof. solve_proper_prepare. repeat f_equiv;auto. Qed.
-  Global Instance rcond_contractive (P : D) (C : CmptName) (p : Perm) :
+  Global Instance rcond_contractive (P : V) (C : CmptName) (p : Perm) :
     Contractive (λ interp, ▷ rcond P C p interp)%I.
   Proof. solve_contractive. Qed.
 
-  Definition wcond (P : D) (C : CmptName) (interp : D) : iProp Σ :=
+  Definition wcond (P : V) (C : CmptName) (interp : V) : iProp Σ :=
     (□ ∀ (W: WORLD) (w : Word), interp W C w -∗ P W C w).
   Global Instance wcond_ne n :
     Proper ((=) ==> (=)  ==> dist n ==> dist n) wcond.
   Proof. solve_proper_prepare. repeat f_equiv;auto. Qed.
-  Global Instance wcond_contractive (P : D) (C : CmptName) :
+  Global Instance wcond_contractive (P : V) (C : CmptName) :
     Contractive (λ interp, ▷ wcond P C interp)%I.
   Proof. solve_contractive. Qed.
 
 
-  Definition exec_cond
-    (W : WORLD) (C : CmptName)
-    (p : Perm) (g : Locality) (b e : Addr)
-    (interp : D) : iProp Σ :=
-    (∀ a regs W', ⌜a ∈ₐ [[ b , e ]]⌝
-               → future_world g W W'
-               → ▷ interp_expr interp regs W' C (WCap p g b e a))%I.
-  Global Instance exec_cond_ne n :
-    Proper ((=) ==> (=) ==> (=) ==> (=) ==> (=) ==> (=) ==> dist n ==> dist n) exec_cond.
-  Proof. unfold exec_cond. solve_proper. Qed.
-  Global Instance exec_cond_contractive W C b e g p :
-    Contractive (λ interp, exec_cond W C b e g p interp).
-  Proof. solve_contractive. Qed.
+  (* Definition exec_cond *)
+  (*   (stk : STK) *)
+  (*   (W : WORLD) (C : CmptName) *)
+  (*   (p : Perm) (g : Locality) (b e : Addr) *)
+  (*   (interp : D) : iProp Σ := *)
+  (*   (∀ a regs W', ⌜a ∈ₐ [[ b , e ]]⌝ *)
+  (*              → future_world g W W' *)
+  (*              → ▷ interp_expr interp regs stk W' C (WCap p g b e a))%I. *)
+  (* Global Instance exec_cond_ne n : *)
+  (*   Proper ((=) ==> (=) ==> (=) ==> (=) ==> (=) ==> (=) ==> dist n ==> dist n) exec_cond. *)
+  (* Proof. unfold exec_cond. solve_proper. Qed. *)
+  (* Global Instance exec_cond_contractive W C b e g p : *)
+  (*   Contractive (λ interp, exec_cond W C b e g p interp). *)
+  (* Proof. solve_contractive. Qed. *)
 
-  Definition enter_cond (W : WORLD) (C : CmptName) (p : Perm) (g : Locality) (b e a : Addr) (interp : D) : iProp Σ :=
-    (∀ r W', future_world g W W' →
-             (▷ interp_expr interp r W' C (WCap p g b e a))
-               ∗ (▷ interp_expr interp r W' C (WCap p Local b e a))
+  Definition enter_cond
+    (W : WORLD) (C : CmptName)
+    (p : Perm) (g : Locality) (b e a : Addr)
+    (interp : V) (interp_cont : K) : iProp Σ :=
+    (∀ stk wstk W', future_world g W W' →
+             (▷ interp_expr interp interp_cont stk W' C (WCap p g b e a) wstk)
+               ∗ (▷ interp_expr interp interp_cont stk W' C (WCap p Local b e a) wstk)
     )%I.
   Global Instance enter_cond_ne n :
-    Proper ((=) ==> (=) ==> (=) ==> (=) ==> (=) ==> (=) ==> (=) ==> dist n ==> dist n) enter_cond.
-  Proof. unfold enter_cond. solve_proper. Qed.
+    Proper ((=) ==> (=) ==> (=) ==> (=) ==> (=) ==> (=) ==> (=) ==> dist n ==> dist n ==> dist n) enter_cond.
+  Proof. solve_proper. Admitted.
   Global Instance enter_cond_contractive W C p g b e a :
     Contractive (λ interp, enter_cond W C p g b e a interp).
-  Proof.
-    solve_contractive.
-  Qed.
+  Proof. Admitted.
+  (*   solve_contractive. *)
+  (* Qed. *)
 
-  Definition persistent_cond (P:D) := (∀ WCv, Persistent (P WCv.1.1 WCv.1.2  WCv.2)).
+  Definition persistent_cond (P:V) := (∀ WCv, Persistent (P WCv.1.1 WCv.1.2  WCv.2)).
 
   (* interp definitions *)
 
@@ -211,10 +257,10 @@ Section logrel.
   (* For simplicity we might want to have the following statement in valididy of caps.
      However, it is strictly not necessary since it can be derived form full_sts_world *)
 
-  Definition safeC (P : D) :=
+  Definition safeC (P : V) :=
     (λ WCv : WORLD * CmptName * (leibnizO Word), P WCv.1.1 WCv.1.2 WCv.2).
 
-  Definition monoReq (W : WORLD) (C : CmptName) (a : Addr) (p : Perm) (P : D) :=
+  Definition monoReq (W : WORLD) (C : CmptName) (a : Addr) (p : Perm) (P : V) :=
     (match (std W) !! a with
         | Some Temporary =>
             (if isWL p
@@ -224,10 +270,10 @@ Section logrel.
         | _ => True
         end)%I.
 
-  Definition interp_z : D := λne _ _ w, ⌜match w with WInt z => True | _ => False end⌝%I.
-  Definition interp_cap_O : D := λne _ _ _, True%I.
+  Definition interp_z : V := λne _ _ w, ⌜match w with WInt z => True | _ => False end⌝%I.
+  Definition interp_cap_O : V := λne _ _ _, True%I.
 
-  Program Definition interp_sentry (interp : D) : D :=
+  Program Definition interp_sentry (interp : V) : V :=
     λne W C w, (match w with
                 | WSentry p g b e a =>
                     (□ enter_cond W C p g b e a interp)
@@ -235,7 +281,7 @@ Section logrel.
                 end)%I.
   Solve All Obligations with solve_proper.
 
-  Program Definition interp_cap (interp : D) : D :=
+  Program Definition interp_cap (interp : V) : V :=
     λne W C w, (match w with
               | WCap (O _ _) _ _ _ _
               | WCap (BPerm XSR _ _ _) _ _ _ _ (* XRS capabilities are never safe-to-share *)
@@ -243,7 +289,7 @@ Section logrel.
                 => False
               | WCap p g b e a =>
                   [∗ list] a ∈ (finz.seq_between b e),
-                    ∃ (p' : Perm) (P:D),
+                    ∃ (p' : Perm) (P:V),
                       ⌜PermFlowsTo p p'⌝
                       ∧ ⌜persistent_cond P⌝
                       ∧ rel C a p' (safeC P)
@@ -258,19 +304,19 @@ Section logrel.
 
   (* (un)seal permission definitions *)
   (* Note the asymmetry: to seal values, we need to know that we are using a persistent predicate to create a value, whereas we do not need this information when unsealing values (it is provided by the `interp_sb` case). *)
-  Definition safe_to_seal (W : WORLD) (C : CmptName) (interp : D) (b e : OType) : iPropO Σ :=
+  Definition safe_to_seal (W : WORLD) (C : CmptName) (interp : V) (b e : OType) : iPropO Σ :=
     ([∗ list] a ∈ (finz.seq_between b e),
-       ∃ P : D, ⌜persistent_cond P⌝
+       ∃ P : V, ⌜persistent_cond P⌝
                 ∗ (∀ w, future_priv_mono C (safeC P) w)
                 ∗ (seal_pred a (safeC P))
                 ∗ ▷ wcond P C interp)%I.
-  Definition safe_to_unseal (W : WORLD) (C : CmptName) (interp : D) (b e : OType) : iPropO Σ :=
+  Definition safe_to_unseal (W : WORLD) (C : CmptName) (interp : V) (b e : OType) : iPropO Σ :=
     ([∗ list] a ∈ (finz.seq_between b e),
-       ∃ P : D, (∀ w, future_priv_mono C (safeC P) w)
+       ∃ P : V, (∀ w, future_priv_mono C (safeC P) w)
                 ∗ (seal_pred a (safeC P))
                 ∗ ▷ rcond P C RO interp)%I.
 
-  Program Definition interp_sr (interp : D) : D :=
+  Program Definition interp_sr (interp : V) : V :=
     λne W C w, (match w with
     | WSealRange p g b e a =>
     (if permit_seal p then safe_to_seal W C interp b e else True)
@@ -279,7 +325,7 @@ Section logrel.
   Solve All Obligations with solve_proper.
 
   Program Definition interp_sb (W : WORLD) (C : CmptName) (o : OType) (w : Word) :=
-    (∃ (P : D) ,
+    (∃ (P : V) ,
         ⌜persistent_cond P⌝
         ∗ (∀ w, future_priv_mono C (safeC P) w)
         ∗ seal_pred o (safeC P)
@@ -287,9 +333,9 @@ Section logrel.
         ∗ ▷ P W C (borrow w)
     )%I.
 
-  Definition interp_False : D := λne _ _ _, False%I.
+  Definition interp_False : V := λne _ _ _, False%I.
 
-  Program Definition interp1 (interp : D) : D :=
+  Program Definition interp1 (interp : V) : V :=
     (λne W C w,
     match w return _ with
     | WInt _ => interp_z W C w
@@ -354,34 +400,35 @@ Section logrel.
     fixpoint (interp1) W C w ≡ interp1 (fixpoint (interp1)) W C w.
   Proof. exact: (fixpoint_unfold (interp1) W C w). Qed.
 
-  Program Definition interp : D := λne W C w, (fixpoint (interp1)) W C w.
+  Program Definition interp : V := λne W C w, (fixpoint (interp1)) W C w.
   Solve All Obligations with solve_proper.
-  Definition interp_expression (r : Reg) : D := interp_expr interp r.
+  Definition interp_expression : E := interp_expr interp.
   Definition interp_registers : R := interp_reg interp.
+  Definition interp_continuation' : K := interp_cont interp.
 
   Global Instance interp_persistent W C w : Persistent (interp W C w).
   Proof.
-    (* intros. destruct_word w; simpl; rewrite fixpoint_interp1_eq; simpl. *)
-    (* - apply _. *)
-    (* - destruct_perm c ; destruct g; repeat (apply exist_persistent; intros); try apply _. *)
-    (* - destruct (permit_seal sr), (permit_unseal sr); rewrite /safe_to_seal /safe_to_unseal; apply _ . *)
-    (* - apply _. *)
-    (* - apply exist_persistent; intros P. *)
-    (*   unfold Persistent. iIntros "(%Hpers & #Hmono & #Hs & HP & HPborrowed)". *)
-    (*   (* use knowledge about persistence *) *)
-    (*   iAssert (<pers> ▷ P W C (WSealable sb))%I with "[ HP ]" as "HP". *)
-    (*   { iApply later_persistently_1. *)
-    (*     ospecialize (Hpers (W,C,_)); cbn in Hpers. *)
-    (*     by iApply persistent_persistently_2. *)
-    (*   } *)
-    (*   iAssert (<pers> ▷ P W C (borrow (WSealable sb)))%I with "[ HPborrowed ]" as "HPborrowed". *)
-    (*   { iApply later_persistently_1. *)
-    (*     ospecialize (Hpers (W,C,_)); cbn in Hpers. *)
-    (*     by iApply persistent_persistently_2. *)
-    (*   } *)
-    (*   iApply persistently_sep_2; iSplitR; auto. *)
-    (*   iApply persistently_sep_2; iSplitR; auto; iFrame "Hs". *)
-    (*   iApply persistently_sep_2;iFrame. *)
+    intros. destruct_word w; simpl; rewrite fixpoint_interp1_eq; simpl.
+    - apply _.
+    - destruct_perm c ; destruct g; repeat (apply exist_persistent; intros); try apply _.
+    - destruct (permit_seal sr), (permit_unseal sr); rewrite /safe_to_seal /safe_to_unseal; apply _ .
+    - apply _.
+    - apply exist_persistent; intros P.
+      unfold Persistent. iIntros "(%Hpers & #Hmono & #Hs & HP & HPborrowed)".
+      (* use knowledge about persistence *)
+      iAssert (<pers> ▷ P W C (WSealable sb))%I with "[ HP ]" as "HP".
+      { iApply later_persistently_1.
+        ospecialize (Hpers (W,C,_)); cbn in Hpers.
+        by iApply persistent_persistently_2.
+      }
+      iAssert (<pers> ▷ P W C (borrow (WSealable sb)))%I with "[ HPborrowed ]" as "HPborrowed".
+      { iApply later_persistently_1.
+        ospecialize (Hpers (W,C,_)); cbn in Hpers.
+        by iApply persistent_persistently_2.
+      }
+      iApply persistently_sep_2; iSplitR; auto.
+      iApply persistently_sep_2; iSplitR; auto; iFrame "Hs".
+      iApply persistently_sep_2;iFrame.
   Admitted. (* TODO holds, but very loooong *)
 
   (* Non-curried version of interp *)
@@ -395,7 +442,7 @@ Section logrel.
           if (has_sreg_access p)
           then False
           else ([∗ list] a ∈ finz.seq_between b e,
-                  ∃ (p' : Perm) (P:D),
+                  ∃ (p' : Perm) (P:V),
                     ⌜PermFlowsTo p p'⌝
                     ∗ ⌜persistent_cond P⌝
                     ∗ rel C a p' (safeC P)
@@ -435,7 +482,7 @@ Section logrel.
     (b ≤ a' ∧ a' < e)%Z →
     readAllowed p →
     ⊢ (interp W C (WCap p g b e a)) →
-    ∃ (p' : Perm) (P:D),
+    ∃ (p' : Perm) (P:V),
       ⌜ PermFlowsTo p p'⌝
       ∗ ⌜persistent_cond P⌝
       ∗ rel C a' p' (safeC P)
@@ -465,7 +512,7 @@ Section logrel.
     (b ≤ a' ∧ a' < e)%Z →
     writeAllowed p →
     ⊢ (interp W C (WCap p g b e a)) →
-    ∃ (p' : Perm) (P:D),
+    ∃ (p' : Perm) (P:V),
       ⌜ PermFlowsTo p p'⌝
       ∗ ⌜persistent_cond P⌝
       ∗ rel C a' p' (safeC P)
@@ -565,7 +612,7 @@ Section logrel.
     (W : WORLD) (C : CmptName)
     (regs : leibnizO Reg) (p : Perm) (g : Locality) (b e a : Addr):
       (∀ (r : RegName) (v : Word), ⌜r ≠ PC⌝ → ⌜regs !! r = Some v⌝ → interp W C v)%I
-    -∗ (∃ (p' : Perm) (P : D),
+    -∗ (∃ (p' : Perm) (P : V),
         ⌜PermFlowsTo p p'⌝
         ∗ ⌜persistent_cond P⌝
         ∗ rel C a p' (safeC P)
@@ -575,7 +622,7 @@ Section logrel.
         ∗ monoReq W C a p' P
         ∗ ⌜if isWL p then region_state_pwl W a else region_state_nwl W a g⌝
        )
-    -∗ (∃ (p' : Perm) (P : D),
+    -∗ (∃ (p' : Perm) (P : V),
         ⌜PermFlowsTo p p'⌝
         ∗ ⌜persistent_cond P⌝
         ∗ rel C a p' (safeC P)
